<?xml version="1.0"?>
<rdf:RDF xmlns="http://ontofox.hegroup.org/ma552mwq.owl#"
     xml:base="http://ontofox.hegroup.org/ma552mwq.owl"
     xmlns:rdf="http://www.w3.org/1999/02/22-rdf-syntax-ns#"
     xmlns:owl="http://www.w3.org/2002/07/owl#"
     xmlns:xsd="http://www.w3.org/2001/XMLSchema#"
     xmlns:rdfs="http://www.w3.org/2000/01/rdf-schema#"
     xmlns:obo="http://purl.obolibrary.org/obo/">
    <owl:Ontology rdf:about="http://ontofox.hegroup.org/ma552mwq.owl"/>
    


    <!-- 
    ///////////////////////////////////////////////////////////////////////////////////////
    //
    // Annotation properties
    //
    ///////////////////////////////////////////////////////////////////////////////////////
     -->

    <owl:AnnotationProperty rdf:about="http://purl.obolibrary.org/obo/IAO_0000412">
        <rdfs:label xml:lang="en">imported from</rdfs:label>
    </owl:AnnotationProperty>
    <owl:AnnotationProperty rdf:about="http://purl.obolibrary.org/obo/IAO_0000115">
        <rdfs:label xml:lang="en">definition</rdfs:label>
        <obo:IAO_0000115 xml:lang="en">The official definition, explaining the meaning of a class or property. Shall be Aristotelian, formalized and normalized. Can be augmented with colloquial definitions.</obo:IAO_0000115>
    </owl:AnnotationProperty>
    <owl:AnnotationProperty rdf:about="http://www.w3.org/2000/01/rdf-schema#label"/>
    


    <!-- 
    ///////////////////////////////////////////////////////////////////////////////////////
    //
    // Datatypes
    //
    ///////////////////////////////////////////////////////////////////////////////////////
     -->

    


    <!-- 
    ///////////////////////////////////////////////////////////////////////////////////////
    //
    // Object Properties
    //
    ///////////////////////////////////////////////////////////////////////////////////////
     -->

    


    <!-- http://purl.obolibrary.org/obo/IAO_0000136 -->

    <owl:ObjectProperty rdf:about="http://purl.obolibrary.org/obo/IAO_0000136">
        <rdfs:label xml:lang="en">is about</rdfs:label>
        <obo:IAO_0000115 xml:lang="en">A (currently) primitive relation that relates an information artifact to an entity.</obo:IAO_0000115>
        <obo:IAO_0000412 rdf:resource="http://purl.obolibrary.org/obo/iao.owl"/>
    </owl:ObjectProperty>
    


    <!-- http://purl.obolibrary.org/obo/IAO_0000219 -->

    <owl:ObjectProperty rdf:about="http://purl.obolibrary.org/obo/IAO_0000219">
        <rdfs:label xml:lang="en">denotes</rdfs:label>
        <obo:IAO_0000115 xml:lang="en">A primitive, instance-level, relation obtaining between an information content entity and some portion of reality. Denotation is what happens when someone creates an information content entity E in order to specifically refer to something. The only relation between E and the thing is that E can be used to &#39;pick out&#39; the thing. This relation connects those two together. Freedictionary.com sense 3: To signify directly; refer to specifically</obo:IAO_0000115>
        <rdfs:subPropertyOf rdf:resource="http://purl.obolibrary.org/obo/IAO_0000136"/>
        <obo:IAO_0000412 rdf:resource="http://purl.obolibrary.org/obo/iao.owl"/>
    </owl:ObjectProperty>
    


    <!-- 
    ///////////////////////////////////////////////////////////////////////////////////////
    //
    // Classes
    //
    ///////////////////////////////////////////////////////////////////////////////////////
     -->

    


    <!-- http://purl.obolibrary.org/obo/BFO_0000001 -->

    <owl:Class rdf:about="http://purl.obolibrary.org/obo/BFO_0000001">
        <rdfs:label xml:lang="en">entity</rdfs:label>
        <obo:IAO_0000412 rdf:resource="http://purl.obolibrary.org/obo/iao.owl"/>
    </owl:Class>
    


    <!-- http://purl.obolibrary.org/obo/BFO_0000002 -->

    <owl:Class rdf:about="http://purl.obolibrary.org/obo/BFO_0000002">
        <rdfs:label xml:lang="en">continuant</rdfs:label>
        <rdfs:subClassOf rdf:resource="http://purl.obolibrary.org/obo/BFO_0000001"/>
        <obo:IAO_0000115 xml:lang="en">An entity that exists in full at any time in which it exists at all, persists through time while maintaining its identity and has no temporal parts.</obo:IAO_0000115>
        <obo:IAO_0000412 rdf:resource="http://purl.obolibrary.org/obo/iao.owl"/>
    </owl:Class>
    


    <!-- http://purl.obolibrary.org/obo/BFO_0000031 -->

    <owl:Class rdf:about="http://purl.obolibrary.org/obo/BFO_0000031">
        <rdfs:label xml:lang="en">generically dependent continuant</rdfs:label>
        <rdfs:subClassOf rdf:resource="http://purl.obolibrary.org/obo/BFO_0000002"/>
        <obo:IAO_0000115 xml:lang="en">A continuant that is dependent on one or other independent continuant bearers. For every instance of A requires some instance of (an independent continuant type) B but which instance of B serves can change from time to time.</obo:IAO_0000115>
        <obo:IAO_0000115 xml:lang="en">b is a generically dependent continuant = Def. b is a continuant that g-depends_on one or more other entities. (axiom label in BFO2 Reference: [074-001])</obo:IAO_0000115>
        <obo:IAO_0000412 rdf:resource="http://purl.obolibrary.org/obo/iao.owl"/>
    </owl:Class>
    


    <!-- http://purl.obolibrary.org/obo/IAO_0000003 -->

    <owl:Class rdf:about="http://purl.obolibrary.org/obo/IAO_0000003">
        <rdfs:label xml:lang="en">measurement unit label</rdfs:label>
        <rdfs:subClassOf rdf:resource="http://purl.obolibrary.org/obo/IAO_0000009"/>
        <obo:IAO_0000115 xml:lang="en">A measurement unit label is as a label that is part of a scalar measurement datum and denotes a unit of measure.</obo:IAO_0000115>
        <obo:IAO_0000412 rdf:resource="http://purl.obolibrary.org/obo/iao.owl"/>
    </owl:Class>
    


    <!-- http://purl.obolibrary.org/obo/IAO_0000005 -->

    <owl:Class rdf:about="http://purl.obolibrary.org/obo/IAO_0000005">
        <rdfs:label xml:lang="en">objective specification</rdfs:label>
        <rdfs:subClassOf rdf:resource="http://purl.obolibrary.org/obo/IAO_0000033"/>
        <obo:IAO_0000115 xml:lang="en">A directive information entity that describes an intended process endpoint. When part of a plan specification the concretization is realized in a planned process in which the bearer tries to effect the world so that the process endpoint is achieved.</obo:IAO_0000115>
        <obo:IAO_0000412 rdf:resource="http://purl.obolibrary.org/obo/iao.owl"/>
    </owl:Class>
    


    <!-- http://purl.obolibrary.org/obo/IAO_0000007 -->

    <owl:Class rdf:about="http://purl.obolibrary.org/obo/IAO_0000007">
        <rdfs:label xml:lang="en">action specification</rdfs:label>
        <rdfs:subClassOf rdf:resource="http://purl.obolibrary.org/obo/IAO_0000033"/>
        <obo:IAO_0000115 xml:lang="en">A directive information entity that describes an action the bearer will take.</obo:IAO_0000115>
        <obo:IAO_0000412 rdf:resource="http://purl.obolibrary.org/obo/iao.owl"/>
    </owl:Class>
    


    <!-- http://purl.obolibrary.org/obo/IAO_0000009 -->

    <owl:Class rdf:about="http://purl.obolibrary.org/obo/IAO_0000009">
        <rdfs:label xml:lang="en">datum label</rdfs:label>
        <rdfs:subClassOf rdf:resource="http://purl.obolibrary.org/obo/IAO_0000030"/>
        <obo:IAO_0000115 xml:lang="en">A label is a symbol that is part of some other datum and is used to either partially define  the denotation of that datum or to provide a means for identifying the datum as a member of the set of data with the same label</obo:IAO_0000115>
        <obo:IAO_0000412 rdf:resource="http://purl.obolibrary.org/obo/iao.owl"/>
    </owl:Class>
    


    <!-- http://purl.obolibrary.org/obo/IAO_0000027 -->

    <owl:Class rdf:about="http://purl.obolibrary.org/obo/IAO_0000027">
        <rdfs:label xml:lang="en">data item</rdfs:label>
        <rdfs:subClassOf rdf:resource="http://purl.obolibrary.org/obo/IAO_0000030"/>
        <obo:IAO_0000115 xml:lang="en">An information content entity that is intended to be a truthful statement about something (modulo, e.g., measurement precision or other systematic errors) and is constructed/acquired by a method which reliably tends to produce (approximately) truthful statements.</obo:IAO_0000115>
        <obo:IAO_0000412 rdf:resource="http://purl.obolibrary.org/obo/iao.owl"/>
    </owl:Class>
    


    <!-- http://purl.obolibrary.org/obo/IAO_0000030 -->

    <owl:Class rdf:about="http://purl.obolibrary.org/obo/IAO_0000030">
        <rdfs:label xml:lang="en">information content entity</rdfs:label>
        <rdfs:subClassOf rdf:resource="http://purl.obolibrary.org/obo/BFO_0000031"/>
        <obo:IAO_0000115 xml:lang="en">A generically dependent continuant that is about some thing.</obo:IAO_0000115>
        <obo:IAO_0000412 rdf:resource="http://purl.obolibrary.org/obo/iao.owl"/>
    </owl:Class>
    


    <!-- http://purl.obolibrary.org/obo/IAO_0000032 -->

    <owl:Class rdf:about="http://purl.obolibrary.org/obo/IAO_0000032">
        <rdfs:label xml:lang="en">scalar measurement datum</rdfs:label>
        <rdfs:subClassOf rdf:resource="http://purl.obolibrary.org/obo/IAO_0000109"/>
        <obo:IAO_0000115 xml:lang="en">A scalar measurement datum is a measurement datum that is composed of two parts, numerals and a unit label.</obo:IAO_0000115>
        <obo:IAO_0000412 rdf:resource="http://purl.obolibrary.org/obo/iao.owl"/>
    </owl:Class>
    


    <!-- http://purl.obolibrary.org/obo/IAO_0000033 -->

    <owl:Class rdf:about="http://purl.obolibrary.org/obo/IAO_0000033">
        <rdfs:label xml:lang="en">directive information entity</rdfs:label>
        <rdfs:subClassOf rdf:resource="http://purl.obolibrary.org/obo/IAO_0000030"/>
        <obo:IAO_0000115 xml:lang="en">An information content entity whose concretizations indicate to their bearer how to realize them in a process.</obo:IAO_0000115>
        <obo:IAO_0000412 rdf:resource="http://purl.obolibrary.org/obo/iao.owl"/>
    </owl:Class>
    


    <!-- http://purl.obolibrary.org/obo/IAO_0000038 -->

    <owl:Class rdf:about="http://purl.obolibrary.org/obo/IAO_0000038">
        <rdfs:label xml:lang="en">graph</rdfs:label>
        <rdfs:subClassOf rdf:resource="http://purl.obolibrary.org/obo/IAO_0000309"/>
        <obo:IAO_0000115 xml:lang="en">A diagram that presents one or more tuples of information by mapping those tuples in to a two dimensional space in a non arbitrary way.</obo:IAO_0000115>
        <obo:IAO_0000412 rdf:resource="http://purl.obolibrary.org/obo/iao.owl"/>
    </owl:Class>
    


    <!-- http://purl.obolibrary.org/obo/IAO_0000101 -->

    <owl:Class rdf:about="http://purl.obolibrary.org/obo/IAO_0000101">
        <rdfs:label xml:lang="en">image</rdfs:label>
        <rdfs:subClassOf rdf:resource="http://purl.obolibrary.org/obo/IAO_0000308"/>
        <obo:IAO_0000115 xml:lang="en">An image is an affine projection to a two dimensional surface, of measurements of some quality of an entity or entities repeated at regular intervals across a spatial range, where the measurements are represented as color and luminosity on the projected on surface.</obo:IAO_0000115>
        <obo:IAO_0000412 rdf:resource="http://purl.obolibrary.org/obo/iao.owl"/>
    </owl:Class>
    


    <!-- http://purl.obolibrary.org/obo/IAO_0000104 -->

    <owl:Class rdf:about="http://purl.obolibrary.org/obo/IAO_0000104">
        <rdfs:label xml:lang="en">plan specification</rdfs:label>
        <rdfs:subClassOf rdf:resource="http://purl.obolibrary.org/obo/IAO_0000033"/>
        <obo:IAO_0000115 xml:lang="en">A directive information entity with action specifications and objective specifications as parts that, when concretized, is realized in a process in which the bearer tries to achieve the objectives by taking the actions specified.</obo:IAO_0000115>
        <obo:IAO_0000412 rdf:resource="http://purl.obolibrary.org/obo/iao.owl"/>
    </owl:Class>
    


    <!-- http://purl.obolibrary.org/obo/IAO_0000109 -->

    <owl:Class rdf:about="http://purl.obolibrary.org/obo/IAO_0000109">
        <rdfs:label xml:lang="en">measurement datum</rdfs:label>
        <rdfs:subClassOf rdf:resource="http://purl.obolibrary.org/obo/IAO_0000027"/>
        <obo:IAO_0000115 xml:lang="en">A measurement datum is an information content entity that is a recording of the output of a measurement such as produced by a device.</obo:IAO_0000115>
        <obo:IAO_0000412 rdf:resource="http://purl.obolibrary.org/obo/iao.owl"/>
    </owl:Class>
    


    <!-- http://purl.obolibrary.org/obo/IAO_0000179 -->

    <owl:Class rdf:about="http://purl.obolibrary.org/obo/IAO_0000179">
        <rdfs:label xml:lang="en">histogram</rdfs:label>
        <rdfs:subClassOf rdf:resource="http://purl.obolibrary.org/obo/IAO_0000038"/>
        <obo:IAO_0000115 xml:lang="en">A histogram is a report graph which is a statistical description of a
distribution in terms of occurrence frequencies of different event classes.</obo:IAO_0000115>
        <obo:IAO_0000412 rdf:resource="http://purl.obolibrary.org/obo/iao.owl"/>
    </owl:Class>
    


    <!-- http://purl.obolibrary.org/obo/IAO_0000308 -->

    <owl:Class rdf:about="http://purl.obolibrary.org/obo/IAO_0000308">
        <rdfs:label xml:lang="en">figure</rdfs:label>
        <rdfs:subClassOf rdf:resource="http://purl.obolibrary.org/obo/IAO_0000030"/>
        <obo:IAO_0000115 xml:lang="en">An information content entity consisting of a two dimensional arrangement of information content entities such that the arrangement itself is about something.</obo:IAO_0000115>
        <obo:IAO_0000412 rdf:resource="http://purl.obolibrary.org/obo/iao.owl"/>
    </owl:Class>
    


    <!-- http://purl.obolibrary.org/obo/IAO_0000309 -->

    <owl:Class rdf:about="http://purl.obolibrary.org/obo/IAO_0000309">
        <rdfs:label xml:lang="en">diagram</rdfs:label>
        <rdfs:subClassOf rdf:resource="http://purl.obolibrary.org/obo/IAO_0000308"/>
        <obo:IAO_0000115 xml:lang="en">A figure that expresses one or more propositions</obo:IAO_0000115>
        <obo:IAO_0000412 rdf:resource="http://purl.obolibrary.org/obo/iao.owl"/>
    </owl:Class>
</rdf:RDF>



<!-- Generated by the OWL API (version 1.3.5.1016) http://owlapi.sourceforge.net -->

