<?xml version="1.0"?>
<rdf:RDF xmlns="http://ontofox.hegroup.org/dsq3wu2n.owl#"
     xml:base="http://ontofox.hegroup.org/dsq3wu2n.owl"
     xmlns:rdf="http://www.w3.org/1999/02/22-rdf-syntax-ns#"
     xmlns:owl="http://www.w3.org/2002/07/owl#"
     xmlns:xsd="http://www.w3.org/2001/XMLSchema#"
     xmlns:rdfs="http://www.w3.org/2000/01/rdf-schema#"
     xmlns:obo="http://purl.obolibrary.org/obo/">
    <owl:Ontology rdf:about="http://ontofox.hegroup.org/dsq3wu2n.owl"/>
    


    <!-- 
    ///////////////////////////////////////////////////////////////////////////////////////
    //
    // Annotation properties
    //
    ///////////////////////////////////////////////////////////////////////////////////////
     -->

    <owl:AnnotationProperty rdf:about="http://purl.obolibrary.org/obo/IAO_0000412">
        <rdfs:label xml:lang="en">imported from</rdfs:label>
    </owl:AnnotationProperty>
    <owl:AnnotationProperty rdf:about="http://purl.obolibrary.org/obo/IAO_0000115">
        <rdfs:label xml:lang="en">definition</rdfs:label>
        <obo:IAO_0000115 xml:lang="en">The official definition, explaining the meaning of a class or property. Shall be Aristotelian, formalized and normalized. Can be augmented with colloquial definitions.</obo:IAO_0000115>
    </owl:AnnotationProperty>
    <owl:AnnotationProperty rdf:about="http://www.w3.org/2000/01/rdf-schema#label">
        <rdfs:label>label</rdfs:label>
    </owl:AnnotationProperty>
    


    <!-- 
    ///////////////////////////////////////////////////////////////////////////////////////
    //
    // Datatypes
    //
    ///////////////////////////////////////////////////////////////////////////////////////
     -->

    


    <!-- 
    ///////////////////////////////////////////////////////////////////////////////////////
    //
    // Classes
    //
    ///////////////////////////////////////////////////////////////////////////////////////
     -->

    


    <!-- http://purl.obolibrary.org/obo/BFO_0000031 -->

    <owl:Class rdf:about="http://purl.obolibrary.org/obo/BFO_0000031">
        <rdfs:label xml:lang="en">generically dependent continuant</rdfs:label>
        <obo:IAO_0000115 xml:lang="en">A continuant that is dependent on one or other independent continuant bearers. For every instance of A requires some instance of (an independent continuant type) B but which instance of B serves can change from time to time.</obo:IAO_0000115>
        <obo:IAO_0000115 xml:lang="en">b is a generically dependent continuant = Def. b is a continuant that g-depends_on one or more other entities. (axiom label in BFO2 Reference: [074-001])</obo:IAO_0000115>
        <obo:IAO_0000412 rdf:resource="http://purl.obolibrary.org/obo/iao/pno.owl"/>
    </owl:Class>
    


    <!-- http://purl.obolibrary.org/obo/IAO_0000030 -->

    <owl:Class rdf:about="http://purl.obolibrary.org/obo/IAO_0000030">
        <rdfs:label xml:lang="en">information content entity</rdfs:label>
        <rdfs:subClassOf rdf:resource="http://purl.obolibrary.org/obo/BFO_0000031"/>
        <obo:IAO_0000115 xml:lang="en">A generically dependent continuant that is about some thing.</obo:IAO_0000115>
        <obo:IAO_0000412 rdf:resource="http://purl.obolibrary.org/obo/iao/pno.owl"/>
    </owl:Class>
    


    <!-- http://purl.obolibrary.org/obo/IAO_0020000 -->

    <owl:Class rdf:about="http://purl.obolibrary.org/obo/IAO_0020000">
        <rdfs:label xml:lang="en">identifier</rdfs:label>
        <rdfs:subClassOf rdf:resource="http://purl.obolibrary.org/obo/IAO_0000030"/>
        <obo:IAO_0000115 xml:lang="en">An identifier is an information content entity that is the outcome of a dubbing process and is used to refer to one instance of entity shared by a group of people to refer to that individual entity.</obo:IAO_0000115>
        <obo:IAO_0000412 rdf:resource="http://purl.obolibrary.org/obo/iao/pno.owl"/>
    </owl:Class>
    


    <!-- http://purl.obolibrary.org/obo/IAO_0020015 -->

    <owl:Class rdf:about="http://purl.obolibrary.org/obo/IAO_0020015">
        <rdfs:label xml:lang="en">personal name</rdfs:label>
        <rdfs:subClassOf rdf:resource="http://purl.obolibrary.org/obo/IAO_0020000"/>
        <obo:IAO_0000115 xml:lang="en">A personal name is a proper name identifying an individual person.</obo:IAO_0000115>
        <obo:IAO_0000412 rdf:resource="http://purl.obolibrary.org/obo/iao/pno.owl"/>
    </owl:Class>
    


    <!-- http://purl.obolibrary.org/obo/IAO_0020016 -->

    <owl:Class rdf:about="http://purl.obolibrary.org/obo/IAO_0020016">
        <rdfs:label xml:lang="en">given name</rdfs:label>
        <rdfs:subClassOf rdf:resource="http://purl.obolibrary.org/obo/IAO_0020015"/>
        <obo:IAO_0000115 xml:lang="en">A given name, in Western contexts often referred to as a first name, is a personal name that specifies and differentiates between members of a group of individuals, especially in a family, all of whose members usually share the same family name (surname). A given name is purposefully given, usually by a child&#39;s parents at or near birth, in contrast to an inherited one such as a family name</obo:IAO_0000115>
        <obo:IAO_0000412 rdf:resource="http://purl.obolibrary.org/obo/iao/pno.owl"/>
    </owl:Class>
    


    <!-- http://purl.obolibrary.org/obo/IAO_0020017 -->

    <owl:Class rdf:about="http://purl.obolibrary.org/obo/IAO_0020017">
        <rdfs:label xml:lang="en">family name</rdfs:label>
        <rdfs:subClassOf rdf:resource="http://purl.obolibrary.org/obo/IAO_0020015"/>
        <obo:IAO_0000115 xml:lang="en">A family name (in Western contexts often referred to as a surname or last name) is typically a part of a person&#39;s name which has been passed, according to law or custom, from one or both parents to their children.</obo:IAO_0000115>
        <obo:IAO_0000412 rdf:resource="http://purl.obolibrary.org/obo/iao/pno.owl"/>
    </owl:Class>
</rdf:RDF>



<!-- Generated by the OWL API (version 1.3.5.1016) http://owlapi.sourceforge.net -->

